theory/bpfConsistencyAux.thy
@@ -3,106 +3,10 @@ theory bpfConsistencyAux
   x64Assembler x64DecodeProof Mem JITCommType
 begin
 
-(*lemma "bop = BPF_ADD \<Longrightarrow> xop = Paddl_rr \<Longrightarrow> *)
-
-(*u8_of_ireg rd = ucast(bpf_ireg2u4 dst) \<Longrightarrow>
-u8_of_ireg ri = ucast(bpf_ireg2u4 src) \<Longrightarrow>*)
-
-
-
-lemma addl_subgoal_rr:
-      "bins = BPF_ALU BPF_ADD dst (SOReg src) \<Longrightarrow>
-       xins = Paddl_rr rd ri \<Longrightarrow>
-       (BPF_OK pc rs' m' ss' is_v1 (cur_cu+1) remain_cu) = step fuel bins rs m ss is_v1 cur_cu remain_cu \<Longrightarrow>
-       Next reg' m'  = exec_instr xins sz reg m \<Longrightarrow> 
-       rd = bpf_to_x64_reg dst \<Longrightarrow>
-       ri = bpf_to_x64_reg src \<Longrightarrow>
-       reg (IR rd) = Vint n1 \<Longrightarrow>
-       reg (IR ri) = Vint n2 \<Longrightarrow>
-       ucast n1 = rs dst \<Longrightarrow>
-       ucast n2  = rs src \<Longrightarrow>
-       reg' (IR rd) = Vint n3 \<Longrightarrow>
-       ucast n3 = rs'dst"
-  apply (unfold exec_instr_def step)
-  apply simp
-  apply (unfold eval_alu32_def)
-  apply (cases BPF_ADD, simp_all)
-  apply (unfold eval_alu32_aux1_def)
-  apply (unfold Let_def)
-  apply (cases BPF_ADD, simp_all)
-  apply (unfold add64_def add32_def)
-  apply (unfold nextinstr_nf_def nextinstr_def eval_reg_def)
-  apply simp
-  apply (unfold add64_def)
-  apply (erule conjE)
-  using cast_lemma1
-  by metis
-
-
-lemma addl_subgoal_ri:
-      "bins = BPF_ALU BPF_ADD dst (SOImm src) \<Longrightarrow>
-       xins = Paddl_ri rd imm \<Longrightarrow>
-       (BPF_OK pc rs' m' ss' is_v1 (cur_cu+1) remain_cu) = step fuel bins rs m ss is_v1 cur_cu remain_cu \<Longrightarrow>
-       Next reg' m' = exec_instr xins sz reg m \<Longrightarrow> 
-       rd = bpf_to_x64_reg dst \<Longrightarrow>
-       imm = ucast (src) \<Longrightarrow>
-       reg (IR rd) = Vint n1 \<Longrightarrow>
-       ucast n1  = rs dst \<Longrightarrow>
-       reg' (IR rd) = Vint n3 \<Longrightarrow>
-       ucast n3 = rs'dst"
-  apply (unfold exec_instr_def step)
-  apply simp
-  apply (unfold eval_alu32_def)
-  apply (cases BPF_ADD, simp_all)
-  apply (unfold eval_alu32_aux1_def)
-  apply (unfold Let_def)
-  apply (cases BPF_ADD, simp_all)
-  apply (unfold add64_def add32_def)
-  apply (unfold nextinstr_nf_def nextinstr_def eval_reg_def)
-  apply simp
-  apply (unfold add64_def)
-  apply (erule conjE)
-  using cast_lemma2 
-  by metis
-
-
-lemma addq_subgoal_rr:
-      "bins = BPF_ALU64 BPF_ADD dst (SOReg src) \<Longrightarrow>
-       xins = Paddq_rr rd ri \<Longrightarrow>
-       (BPF_OK pc rs' m' ss' is_v1 (cur_cu+1) remain_cu) = step fuel bins rs m ss is_v1 cur_cu remain_cu \<Longrightarrow>
-       Next reg' m'  = exec_instr xins sz reg m \<Longrightarrow> 
-       corr_registers dst rd \<Longrightarrow>
-       corr_registers src ri \<Longrightarrow>
-       reg (IR rd) = Vlong n1 \<Longrightarrow>
-       reg (IR ri) = Vlong n2 \<Longrightarrow>
-       n1  = rs dst \<Longrightarrow>
-       n2  = rs src \<Longrightarrow>
-       reg' (IR rd) = Vlong n3 \<Longrightarrow>
-       ucast n3 = rs'dst"
-  apply (unfold exec_instr_def step)
-  apply simp
-  apply (unfold eval_alu64_def)
-  apply (cases BPF_ADD, simp_all)
-  apply (unfold add64_def)
-  apply (unfold nextinstr_nf_def nextinstr_def eval_reg_def)
-  apply simp
-  apply (erule conjE)
-  apply (cases "is_v1 cur_cu remain_cu", simp_all)
-  apply(cases "dst = BR10")
-  apply auto[1]
-  apply (cases "is_v1 cur_cu remain_cu", simp_all)
-  apply(cases "dst = BR10", simp_all)
-  apply auto[1]
-    (*ADD64, stack pointer*)
-  sorry
- 
-
-
 
 (*
 definition rel_reg :: "bpf_ireg => ireg => bool" where
 "rel_reg br ir = " *)
-
 
 (*
 Inductive star (ge: genv): state -> trace -> state -> Prop :=
@@ -141,13 +45,590 @@ fun exec_instrs :: "instruction list \<Rightarrow> outcome \<Rightarrow> outcome
     exec_instrs t st1
 )" 
 
-(**r 
-definition per_jit_sub_reg64 :: "bpf_ireg => bpf_ireg => x64_bin"
+(*
+  BPF_DIV, BPF_MOD,  
+  BPF_LSH, BPF_RSH,
+  BPF_ARSH 
+*)
 
-per_jit_sub_reg64 dst src = bl \<Longrightarrow> (**r JIT + x64_encode *)
-x64decode bl = Some (sz, xins) \<Longrightarrow>
+subsection    \<open> BPF_ALU64 auxs\<close> 
+
+lemma aluq_subgoal_rr_aux1:
+     "op1 \<in> {BPF_SUB, BPF_ADD, BPF_MOV, BPF_AND, BPF_XOR, BPF_OR} \<Longrightarrow>
+     bins = BPF_ALU64 op1 dst (SOReg src) \<Longrightarrow>
+     xins = (let op2 = (case op1 of 
+        BPF_SUB \<Rightarrow> Psubq_rr | BPF_ADD \<Rightarrow> Paddq_rr | BPF_MOV \<Rightarrow> Pmovq_rr | BPF_AND \<Rightarrow> Pandq_rr | BPF_XOR \<Rightarrow> Pxorq_rr | 
+        BPF_OR \<Rightarrow> Porq_rr ) in op2 rd ri) \<Longrightarrow>
+     (BPF_OK pc rs' m' ss' is_v1 (cur_cu+1) remain_cu) = step fuel bins rs m ss is_v1 cur_cu remain_cu \<Longrightarrow>
+     Next reg' m' = exec_instr xins sz reg m \<Longrightarrow>
+     rd = (bpf_to_x64_reg dst) \<Longrightarrow>
+     ri = (bpf_to_x64_reg src) \<Longrightarrow>
+     reg (IR rd) = Vlong n1 \<Longrightarrow>
+     reg (IR ri) = Vlong n2 \<Longrightarrow>
+     n1  = rs dst \<Longrightarrow>
+     n2  = rs src \<Longrightarrow> 
+     Vlong (rs' dst) = reg' (IR (bpf_to_x64_reg dst))"
+  apply (unfold exec_instr_def step)
+  apply simp
+  apply(cases op1,simp_all)
+  apply (unfold eval_alu64_def eval_alu64_aux1_def eval_alu64_aux2_def Let_def)
+  apply (unfold sub64_def add64_def and64_def xor64_def or64_def)
+  apply (unfold nextinstr_nf_def nextinstr_def eval_reg_def)
+  by simp_all
+
+lemma aluq_subgoal_rr_aux2_1:"op1 \<in> {Psubq_rr, Pmovq_rr,Paddq_rr, Pandq_rr, Pxorq_rr, Porq_rr} \<Longrightarrow> 
+    xins = op1 dst src \<Longrightarrow> Next reg' m' = exec_instr xins sz reg m \<Longrightarrow> 
+    \<forall> r\<noteq>dst. reg' (IR r) = reg (IR r)"
+  apply(unfold exec_instr_def, cases "xins", simp_all)
+  apply(unfold nextinstr_nf_def nextinstr_def add64_def sub64_def and64_def xor64_def or64_def) 
+  by auto
+
+lemma aluq_subgoal_rr_aux2_2:"op1 \<in> {Psubq_rr, Pmovq_rr, Paddq_rr, Pandq_rr, Pxorq_rr, Porq_rr} \<Longrightarrow> 
+    xins = op1 (bpf_to_x64_reg dst) (bpf_to_x64_reg src) \<Longrightarrow> Next reg' m' = exec_instr xins sz reg m \<Longrightarrow>
+    \<forall> r \<noteq> bpf_to_x64_reg dst. reg' (IR r) = reg (IR r)"
+  using aluq_subgoal_rr_aux2_1 by blast
+
+lemma aluq_subgoal_rr_aux2:"op1 \<in> {Psubq_rr, Pmovq_rr, Paddq_rr, Pandq_rr, Pxorq_rr, Porq_rr} \<Longrightarrow> xins = op1 (bpf_to_x64_reg dst) (bpf_to_x64_reg src) \<Longrightarrow> Next reg' m' = exec_instr xins sz reg m \<Longrightarrow>
+       \<forall> r \<noteq> dst. reg' (IR (bpf_to_x64_reg r)) = reg (IR (bpf_to_x64_reg r))"
+  using bpf_to_x64_reg_corr aluq_subgoal_rr_aux2_2 by metis
+
+lemma aluq_subgoal_rr_aux3:"op2 \<in> {BPF_SUB, BPF_MOV, BPF_ADD, BPF_AND, BPF_XOR, BPF_OR} \<Longrightarrow>
+    bins = BPF_ALU64 op2 dst (SOReg src) \<Longrightarrow> (BPF_OK pc rs' m' ss' is_v1 (cur_cu+1) remain_cu) = step fuel bins rs m ss is_v1 cur_cu remain_cu \<Longrightarrow>
+    \<forall> r \<noteq> dst. rs' r = rs r"
+  apply(cases "bins",simp_all)
+  apply(cases op2)
+  apply(unfold eval_alu64_def,simp)
+  by (unfold eval_alu64_aux1_def, simp_all)
+
+(*
+lemma addq_subgoal_rr:
+      "bins = BPF_ALU64 BPF_ADD dst (SOReg src) \<Longrightarrow>
+       xins = Paddq_rr rd ri \<Longrightarrow>
+       (BPF_OK pc rs' m' ss' is_v1 (cur_cu+1) remain_cu) = step fuel bins rs m ss is_v1 cur_cu remain_cu \<Longrightarrow>
+       Next reg' m' = exec_instr xins sz reg m \<Longrightarrow> 
+       rd = bpf_to_x64_reg dst \<Longrightarrow>
+       ri = bpf_to_x64_reg src \<Longrightarrow>
+       reg (IR rd) = Vlong n1 \<Longrightarrow>
+       reg (IR ri) = Vlong n2 \<Longrightarrow>
+       n1  = rs dst \<Longrightarrow>
+       n2  = rs src \<Longrightarrow>
+       Vlong (rs' dst) = reg' (IR (bpf_to_x64_reg dst))"
+  apply (unfold exec_instr_def step,simp_all)
+  apply (unfold eval_alu64_def)
+  apply (cases BPF_ADD, simp_all)
+  apply (unfold add64_def eval_alu64_aux1_def Let_def)
+  apply (cases BPF_ADD)
+  apply (unfold nextinstr_nf_def nextinstr_def eval_reg_def)
+  by simp_all
+
+lemma addq_subgoal_rr_aux2_1:"xins = Paddq_rr dst src \<Longrightarrow> Next reg' m' = exec_instr xins sz reg m \<Longrightarrow> \<forall> r \<noteq> dst . reg' (IR r) = reg (IR r)"
+  apply(unfold exec_instr_def, cases "xins", simp_all)
+  apply(unfold nextinstr_nf_def nextinstr_def add64_def) 
+  by auto
+
+lemma addq_subgoal_rr_aux2_2:"xins = Paddq_rr (bpf_to_x64_reg dst) (bpf_to_x64_reg src) \<Longrightarrow> Next reg' m' = exec_instr xins sz reg m \<Longrightarrow>
+       \<forall> r \<noteq> bpf_to_x64_reg dst. reg' (IR r) = reg (IR r)"
+  using addq_subgoal_rr_aux2_1 by blast
+
+lemma addq_subgoal_rr_aux2:"xins = Paddq_rr (bpf_to_x64_reg dst) (bpf_to_x64_reg src) \<Longrightarrow> Next reg' m' = exec_instr xins sz reg m \<Longrightarrow>
+       \<forall> r \<noteq> dst. reg' (IR (bpf_to_x64_reg r)) = reg (IR (bpf_to_x64_reg r))"
+  using bpf_to_x64_reg_corr addq_subgoal_rr_aux2_2 by metis
+
+lemma addq_subgoal_rr_aux3:"bins = BPF_ALU64 BPF_ADD dst (SOReg src) \<Longrightarrow> (BPF_OK pc rs' m' ss' is_v1 (cur_cu+1) remain_cu) = step fuel bins rs m ss is_v1 cur_cu remain_cu \<Longrightarrow>
+       \<forall> r \<noteq> dst. rs' r = rs r"
+  apply(cases "bins",simp_all)
+  apply(unfold eval_alu64_def,simp)
+  by (unfold eval_alu64_aux1_def, simp)
 
 *)
+
+subsubsection   \<open> BPF_ALU64 ADD64\<close>  
+
+lemma addq_subgoal_rr_generic:
+  assumes a0:"bins = BPF_ALU64 BPF_ADD dst (SOReg src)" and
+       a1:"per_jit_add_reg64_1 dst src = Some bl" and
+       a2:"list_in_list bl (unat pc) l_bin" and
+       a3:"x64_decode (unat pc) l_bin = Some (length l_bin, xins)" and
+       a4:"(BPF_OK pc rs' m' ss' is_v1 (cur_cu+1) remain_cu) = step fuel bins rs m ss is_v1 cur_cu remain_cu" and
+       a5:"Next reg' m'  = exec_instr xins sz reg m" and
+       a6:"(\<forall> r. Vlong (rs r) = reg (IR (bpf_to_x64_reg r)))" 
+  shows "(\<forall> r. Vlong (rs' r) = reg' (IR (bpf_to_x64_reg r)))"
+proof -
+  have b0:"xins = Paddq_rr (bpf_to_x64_reg dst) (bpf_to_x64_reg src)" using x64_encode_decode_consistency per_jit_add_reg64_1_def a1 a2 a3 by fastforce
+    moreover have b1:"Vlong (rs dst) = reg (IR (bpf_to_x64_reg dst))" using a6 spec by simp
+    moreover have b2:"Vlong (rs src) = reg (IR (bpf_to_x64_reg src))" using a6 spec by simp
+    hence b3:"Vlong (rs' dst) = reg' (IR (bpf_to_x64_reg dst))" using aluq_subgoal_rr_aux1 b0 b1 b2 a0 a4 a5 by force
+    have b4:"\<forall> r \<noteq> dst. reg'(IR (bpf_to_x64_reg r)) = reg (IR (bpf_to_x64_reg r))" using b0 a5 aluq_subgoal_rr_aux2 by blast
+    have b5:"\<forall> r \<noteq> dst. Vlong (rs' r) = Vlong (rs r)" using a0 a4 aluq_subgoal_rr_aux3 by blast
+    have b6:"\<forall> r \<noteq> dst. Vlong (rs r) = reg (IR (bpf_to_x64_reg r))" using a6 by blast
+    have b7:"(\<forall> r \<noteq> dst. Vlong (rs' r) = reg' (IR (bpf_to_x64_reg r)))" by(simp add:b4 b5 b6) 
+    thus ?thesis using b3 by fastforce
+  qed
+
+
+subsubsection   \<open> BPF_ALU64 SUB64\<close> 
+
+lemma subq_subgoal_rr_generic:
+  assumes a0:"bins = BPF_ALU64 BPF_SUB dst (SOReg src)" and
+       a1:"per_jit_sub_reg64 dst src = Some bl" and
+       a2:"list_in_list bl (unat pc) l_bin" and
+       a3:"x64_decode (unat pc) l_bin = Some (length l_bin, xins)" and
+       a4:"(BPF_OK pc rs' m' ss' is_v1 (cur_cu+1) remain_cu) = step fuel bins rs m ss is_v1 cur_cu remain_cu" and
+       a5:"Next reg' m'  = exec_instr xins sz reg m" and
+       a6:"(\<forall> r. Vlong (rs r) = reg (IR (bpf_to_x64_reg r)))" 
+  shows "(\<forall> r. Vlong (rs' r) = reg' (IR (bpf_to_x64_reg r)))"
+proof -
+  have b0:"xins = Psubq_rr (bpf_to_x64_reg dst) (bpf_to_x64_reg src)" using x64_encode_decode_consistency per_jit_sub_reg64_def a1 a2 a3 by fastforce
+    moreover have b1:"Vlong (rs dst) = reg (IR (bpf_to_x64_reg dst))" using a6 spec by simp
+    moreover have b2:"Vlong (rs src) = reg (IR (bpf_to_x64_reg src))" using a6 spec by simp
+    hence b3:"Vlong (rs' dst) = reg' (IR (bpf_to_x64_reg dst))" using aluq_subgoal_rr_aux1 b0 b1 b2 a0 a4 a5 by force
+    have b4:"\<forall> r \<noteq> dst. reg'(IR (bpf_to_x64_reg r)) = reg (IR (bpf_to_x64_reg r))" using b0 a5 aluq_subgoal_rr_aux2 by blast
+    have b5:"\<forall> r \<noteq> dst. Vlong (rs' r) = Vlong (rs r)" using a0 a4 aluq_subgoal_rr_aux3 by blast
+    have b6:"\<forall> r \<noteq> dst. Vlong (rs r) = reg (IR (bpf_to_x64_reg r))" using a6 by blast
+    have b7:"(\<forall> r \<noteq> dst. Vlong (rs' r) = reg' (IR (bpf_to_x64_reg r)))" by(simp add:b4 b5 b6) 
+    thus ?thesis using b3 by fastforce
+  qed
+
+subsubsection   \<open> BPF_ALU64 AND64\<close>
+
+lemma andq_subgoal_rr_generic:
+  assumes a0:"bins = BPF_ALU64 BPF_AND dst (SOReg src)" and
+       a1:"per_jit_and_reg64 dst src = Some bl" and
+       a2:"list_in_list bl (unat pc) l_bin" and
+       a3:"x64_decode (unat pc) l_bin = Some (length l_bin, xins)" and
+       a4:"(BPF_OK pc rs' m' ss' is_v1 (cur_cu+1) remain_cu) = step fuel bins rs m ss is_v1 cur_cu remain_cu" and
+       a5:"Next reg' m'  = exec_instr xins sz reg m" and
+       a6:"(\<forall> r. Vlong (rs r) = reg (IR (bpf_to_x64_reg r)))" 
+  shows "(\<forall> r. Vlong (rs' r) = reg' (IR (bpf_to_x64_reg r)))"
+proof -
+  have b0:"xins = Pandq_rr (bpf_to_x64_reg dst) (bpf_to_x64_reg src)" using x64_encode_decode_consistency per_jit_and_reg64_def a1 a2 a3 by fastforce
+    moreover have b1:"Vlong (rs dst) = reg (IR (bpf_to_x64_reg dst))" using a6 spec by simp
+    moreover have b2:"Vlong (rs src) = reg (IR (bpf_to_x64_reg src))" using a6 spec by simp
+    hence b3:"Vlong (rs' dst) = reg' (IR (bpf_to_x64_reg dst))" using aluq_subgoal_rr_aux1 b0 b1 b2 a0 a4 a5 by force
+    have b4:"\<forall> r \<noteq> dst. reg'(IR (bpf_to_x64_reg r)) = reg (IR (bpf_to_x64_reg r))" using b0 a5 aluq_subgoal_rr_aux2 by blast
+    have b5:"\<forall> r \<noteq> dst. Vlong (rs' r) = Vlong (rs r)" using a0 a4 aluq_subgoal_rr_aux3 by blast
+    have b6:"\<forall> r \<noteq> dst. Vlong (rs r) = reg (IR (bpf_to_x64_reg r))" using a6 by blast
+    have b7:"(\<forall> r \<noteq> dst. Vlong (rs' r) = reg' (IR (bpf_to_x64_reg r)))" by(simp add:b4 b5 b6) 
+    thus ?thesis using b3 by fastforce
+  qed
+
+(*
+lemma subq_subgoal_rr_aux1:
+     "bins = BPF_ALU64 BPF_SUB dst (SOReg src) \<Longrightarrow>
+     xins = Psubq_rr rd ri \<Longrightarrow>
+     (BPF_OK pc rs' m' ss' is_v1 (cur_cu+1) remain_cu) = step fuel bins rs m ss is_v1 cur_cu remain_cu \<Longrightarrow>
+     Next reg' m' = exec_instr xins sz reg m \<Longrightarrow>
+     rd = (bpf_to_x64_reg dst) \<Longrightarrow>
+     ri = (bpf_to_x64_reg src) \<Longrightarrow>
+     reg (IR rd) = Vlong n1 \<Longrightarrow>
+     reg (IR ri) = Vlong n2 \<Longrightarrow>
+     n1  = rs dst \<Longrightarrow>
+     n2  = rs src \<Longrightarrow> 
+     Vlong (rs' dst) = reg' (IR (bpf_to_x64_reg dst))"
+  apply (unfold exec_instr_def step)
+  apply simp
+  apply (unfold eval_alu64_def)
+  apply (cases BPF_SUB, simp_all)
+  apply (unfold eval_alu64_aux1_def)
+  apply (unfold Let_def)
+  apply (cases BPF_SUB, simp_all)
+  apply (unfold sub64_def)
+  apply (unfold nextinstr_nf_def nextinstr_def eval_reg_def)
+  by simp
+
+lemma subq_subgoal_rr_aux2_1:"xins = Psubq_rr dst src \<Longrightarrow> Next reg' m' = exec_instr xins sz reg m \<Longrightarrow> \<forall> r \<noteq> dst . reg' (IR r) = reg (IR r)"
+  apply(unfold exec_instr_def, cases "xins", simp_all)
+  apply(unfold nextinstr_nf_def nextinstr_def add64_def) 
+  by auto
+
+lemma subq_subgoal_rr_aux2_2:"xins = Psubq_rr (bpf_to_x64_reg dst) (bpf_to_x64_reg src) \<Longrightarrow> Next reg' m' = exec_instr xins sz reg m \<Longrightarrow>
+       \<forall> r \<noteq> bpf_to_x64_reg dst. reg' (IR r) = reg (IR r)"
+  using subq_subgoal_rr_aux2_1 by blast
+
+lemma subq_subgoal_rr_aux2:"xins = Psubq_rr (bpf_to_x64_reg dst) (bpf_to_x64_reg src) \<Longrightarrow> Next reg' m' = exec_instr xins sz reg m \<Longrightarrow>
+       \<forall> r \<noteq> dst. reg' (IR (bpf_to_x64_reg r)) = reg (IR (bpf_to_x64_reg r))"
+  using bpf_to_x64_reg_corr subq_subgoal_rr_aux2_2 by metis
+
+
+lemma subq_subgoal_rr_aux3:"bins = BPF_ALU64 BPF_SUB dst (SOReg src) \<Longrightarrow> (BPF_OK pc rs' m' ss' is_v1 (cur_cu+1) remain_cu) = step fuel bins rs m ss is_v1 cur_cu remain_cu \<Longrightarrow>
+       \<forall> r \<noteq> dst. rs' r = rs r"
+  apply(cases "bins",simp_all)
+  apply(unfold eval_alu64_def,simp)
+  by (unfold eval_alu64_aux1_def, simp)
+*)
+
+
+subsubsection   \<open> BPF_ALU64 MOV64\<close>
+
+lemma movq_subgoal_rr_generic:
+  assumes a0:"bins = BPF_ALU64 BPF_MOV dst (SOReg src)" and
+       a1:"per_jit_mov_reg64 dst src = Some bl" and
+       a2:"list_in_list bl (unat pc) l_bin" and
+       a3:"x64_decode (unat pc) l_bin = Some (length l_bin, xins)" and
+       a4:"(BPF_OK pc rs' m' ss' is_v1 (cur_cu+1) remain_cu) = step fuel bins rs m ss is_v1 cur_cu remain_cu" and
+       a5:"Next reg' m'  = exec_instr xins sz reg m" and
+       a6:"(\<forall> r. Vlong (rs r) = reg (IR (bpf_to_x64_reg r)))" 
+  shows "(\<forall> r. Vlong (rs' r) = reg' (IR (bpf_to_x64_reg r)))"
+proof -
+  have b0:"xins = Pmovq_rr (bpf_to_x64_reg dst) (bpf_to_x64_reg src)" using x64_encode_decode_consistency per_jit_mov_reg64_def a1 a2 a3 by fastforce
+    moreover have b1:"Vlong (rs dst) = reg (IR (bpf_to_x64_reg dst))" using a6 spec by simp
+    moreover have b2:"Vlong (rs src) = reg (IR (bpf_to_x64_reg src))" using a6 spec by simp
+    hence b3:"Vlong (rs' dst) = reg' (IR (bpf_to_x64_reg dst))" using aluq_subgoal_rr_aux1 b0 b1 b2 a0 a4 a5 by force
+    have b4:"\<forall> r \<noteq> dst. reg'(IR (bpf_to_x64_reg r)) = reg (IR (bpf_to_x64_reg r))" using b0 a5 aluq_subgoal_rr_aux2 by blast
+    have b5:"\<forall> r \<noteq> dst. Vlong (rs' r) = Vlong (rs r)" using a0 a4 aluq_subgoal_rr_aux3 by blast
+    have b6:"\<forall> r \<noteq> dst. Vlong (rs r) = reg (IR (bpf_to_x64_reg r))" using a6 by blast
+    have b7:"(\<forall> r \<noteq> dst. Vlong (rs' r) = reg' (IR (bpf_to_x64_reg r)))" by(simp add:b4 b5 b6) 
+    thus ?thesis using b3 by fastforce
+  qed
+
+
+subsubsection   \<open> BPF_ALU64 XOR64\<close>
+
+lemma xorq_subgoal_rr_generic:
+  assumes a0:"bins = BPF_ALU64 BPF_XOR dst (SOReg src)" and
+       a1:"per_jit_xor_reg64 dst src = Some bl" and
+       a2:"list_in_list bl (unat pc) l_bin" and
+       a3:"x64_decode (unat pc) l_bin = Some (length l_bin, xins)" and
+       a4:"(BPF_OK pc rs' m' ss' is_v1 (cur_cu+1) remain_cu) = step fuel bins rs m ss is_v1 cur_cu remain_cu" and
+       a5:"Next reg' m'  = exec_instr xins sz reg m" and
+       a6:"(\<forall> r. Vlong (rs r) = reg (IR (bpf_to_x64_reg r)))" 
+  shows "(\<forall> r. Vlong (rs' r) = reg' (IR (bpf_to_x64_reg r)))"
+proof -
+  have b0:"xins = Pxorq_rr (bpf_to_x64_reg dst) (bpf_to_x64_reg src)" using x64_encode_decode_consistency per_jit_xor_reg64_def a1 a2 a3 by fastforce
+    moreover have b1:"Vlong (rs dst) = reg (IR (bpf_to_x64_reg dst))" using a6 spec by simp
+    moreover have b2:"Vlong (rs src) = reg (IR (bpf_to_x64_reg src))" using a6 spec by simp
+    hence b3:"Vlong (rs' dst) = reg' (IR (bpf_to_x64_reg dst))" using aluq_subgoal_rr_aux1 b0 b1 b2 a0 a4 a5 by force
+    have b4:"\<forall> r \<noteq> dst. reg'(IR (bpf_to_x64_reg r)) = reg (IR (bpf_to_x64_reg r))" using b0 a5 aluq_subgoal_rr_aux2 by blast
+    have b5:"\<forall> r \<noteq> dst. Vlong (rs' r) = Vlong (rs r)" using a0 a4 aluq_subgoal_rr_aux3 by blast
+    have b6:"\<forall> r \<noteq> dst. Vlong (rs r) = reg (IR (bpf_to_x64_reg r))" using a6 by blast
+    have b7:"(\<forall> r \<noteq> dst. Vlong (rs' r) = reg' (IR (bpf_to_x64_reg r)))" by(simp add:b4 b5 b6) 
+    thus ?thesis using b3 by fastforce
+  qed
+
+subsubsection   \<open> BPF_ALU64 OR64\<close> 
+
+lemma orq_subgoal_rr_generic:
+  assumes a0:"bins = BPF_ALU64 BPF_OR dst (SOReg src)" and
+       a1:"per_jit_or_reg64 dst src = Some bl" and
+       a2:"list_in_list bl (unat pc) l_bin" and
+       a3:"x64_decode (unat pc) l_bin = Some (length l_bin, xins)" and
+       a4:"(BPF_OK pc rs' m' ss' is_v1 (cur_cu+1) remain_cu) = step fuel bins rs m ss is_v1 cur_cu remain_cu" and
+       a5:"Next reg' m'  = exec_instr xins sz reg m" and
+       a6:"(\<forall> r. Vlong (rs r) = reg (IR (bpf_to_x64_reg r)))" 
+  shows "(\<forall> r. Vlong (rs' r) = reg' (IR (bpf_to_x64_reg r)))"
+proof -
+  have b0:"xins = Porq_rr (bpf_to_x64_reg dst) (bpf_to_x64_reg src)" using x64_encode_decode_consistency per_jit_or_reg64_def a1 a2 a3 by fastforce
+    moreover have b1:"Vlong (rs dst) = reg (IR (bpf_to_x64_reg dst))" using a6 spec by simp
+    moreover have b2:"Vlong (rs src) = reg (IR (bpf_to_x64_reg src))" using a6 spec by simp
+    hence b3:"Vlong (rs' dst) = reg' (IR (bpf_to_x64_reg dst))" using aluq_subgoal_rr_aux1 b0 b1 b2 a0 a4 a5 by force
+    have b4:"\<forall> r \<noteq> dst. reg'(IR (bpf_to_x64_reg r)) = reg (IR (bpf_to_x64_reg r))" using b0 a5 aluq_subgoal_rr_aux2 by blast
+    have b5:"\<forall> r \<noteq> dst. Vlong (rs' r) = Vlong (rs r)" using a0 a4 aluq_subgoal_rr_aux3 by blast
+    have b6:"\<forall> r \<noteq> dst. Vlong (rs r) = reg (IR (bpf_to_x64_reg r))" using a6 by blast
+    have b7:"(\<forall> r \<noteq> dst. Vlong (rs' r) = reg' (IR (bpf_to_x64_reg r)))" by(simp add:b4 b5 b6) 
+    thus ?thesis using b3 by fastforce
+  qed
+
+  subsubsection   \<open> BPF_ALU64 SHL64\<close>
+
+
+lemma add_sub_consistency:"add64 (Vlong a) (Vlong b) = Vlong c \<Longrightarrow> sub64 (Vlong c) (Vlong a) = (Vlong b) "
+  using add64_def sub64_def by auto
+
+lemma shift_subgoal_rr_aux1_1:"Next reg'' m'' = interp2 n xins (Next reg m) \<Longrightarrow> length xins = (2::nat) \<Longrightarrow> \<exists> reg' m'. Next reg' m' = (exec_instr (xins!0) 1 reg m) \<and> Next reg'' m'' = (exec_instr (xins!1) 1 reg' m')  "
+  sorry  
+
+lemma shift_subgoal_rr_aux1_2:"length xins = (2::nat) \<Longrightarrow> Next reg' m' = (exec_instr (xins!0) 1 reg m)  \<Longrightarrow> Next reg'' m'' = (exec_instr (xins!1) 1 reg' m')  \<Longrightarrow>
+  Next reg'' m'' = interp2 3 xins (Next reg m)"
+  sorry
+
+lemma shift_subgoal_rr_aux2_1:"xins = Pmovq_rr src (x64Syntax.RCX) \<Longrightarrow> 
+    Next reg'' m'' = (exec_instr xins 1 reg m) \<Longrightarrow> m'' = m "
+  apply(unfold exec_instr_def) by simp
+
+lemma shift_subgoal_rr_aux2_2:"xins = Pshlq_r dst \<Longrightarrow> 
+    Next reg'' m'' = (exec_instr xins 1 reg m) \<Longrightarrow> m'' = m"
+  apply(unfold exec_instr_def) by simp
+
+lemma shift_subgoal_rr_aux2_3:
+  assumes a0:"xins = [(Pmovq_rr src (x64Syntax.RCX)),(Pshlq_r dst)]" and 
+    a1:"Next reg' m' = (exec_instr (xins!0) 1 reg m) " and
+    a2:"Next reg'' m'' = (exec_instr (xins!1) 1 reg' m') " 
+  shows " m'' = m"
+  using shift_subgoal_rr_aux2_1 shift_subgoal_rr_aux2_2 
+  by (metis One_nat_def a0 a1 a2 nth_Cons_0 nth_Cons_Suc)
+
+lemma shift_subgoal_rr_aux2:
+  assumes a0:"xins = [(Pmovq_rr src (x64Syntax.RCX)),(Pshlq_r dst)]" and 
+    a1:"Next reg'' m'' = interp2 n xins (Next reg m) " 
+  shows " m'' = m"
+proof-
+  have b0:"length xins = (2::nat)" using a0 by simp
+  thus ?thesis using b0 a0 a1 shift_subgoal_rr_aux2_3 
+    by (meson shift_subgoal_rr_aux1_1)
+qed
+
+lemma reg_rsp_consist:"dst = (bpf_to_x64_reg r) \<Longrightarrow> dst \<noteq> x64Syntax.RSP"
+  apply(cases r) 
+  by (unfold bpf_to_x64_reg_corr bpf_to_x64_reg_def, simp_all)
+
+lemma shift_subgoal_rr_aux3_1:"xins = Pmovq_rr (bpf_to_x64_reg src) (x64Syntax.RCX) \<Longrightarrow> 
+    Next reg'' m'' = (exec_instr xins 1 reg m) \<Longrightarrow> reg'' (IR SP) = reg (IR SP) "
+  apply(unfold exec_instr_def reg_rsp_consist bpf_to_x64_reg_corr) 
+  using nextinstr_def reg_rsp_consist by fastforce
+
+lemma shift_subgoal_rr_aux3_2:"xins = Pshlq_r (bpf_to_x64_reg dst) \<Longrightarrow> 
+    Next reg'' m'' = (exec_instr xins 1 reg m) \<Longrightarrow> reg'' (IR SP) = reg (IR SP) "
+  apply(unfold exec_instr_def reg_rsp_consist bpf_to_x64_reg_corr) 
+  using nextinstr_def reg_rsp_consist sorry
+
+lemma shift_subgoal_rr_aux3_3:
+  assumes a0:"xins = [(Pmovq_rr (bpf_to_x64_reg src) (x64Syntax.RCX)),(Pshlq_r (bpf_to_x64_reg dst))]" and 
+    a1:"Next reg' m' = (exec_instr (xins!0) 1 reg m) " and
+    a2:"Next reg'' m'' = (exec_instr (xins!1) 1 reg' m') " 
+  shows " reg'' (IR SP) = reg (IR SP) "
+  using shift_subgoal_rr_aux3_1 shift_subgoal_rr_aux3_2 reg_rsp_consist
+  by (metis One_nat_def a0 a1 a2 nth_Cons_0 nth_Cons_Suc)
+
+lemma shift_subgoal_rr_aux3:
+  assumes a0:"xins = [(Pmovq_rr (bpf_to_x64_reg src) (x64Syntax.RCX)),(Pshlq_r (bpf_to_x64_reg dst))]" and 
+    a1:"Next reg'' m'' = interp2 n xins (Next reg m) " 
+  shows "reg'' (IR SP) = reg (IR SP)"
+proof-
+  have b0:"length xins = (2::nat)" using a0 by simp
+  thus ?thesis using b0 a0 a1 shift_subgoal_rr_aux3_3 
+    by (meson shift_subgoal_rr_aux1_1)
+qed
+
+lemma push_pop_subgoal_rr_aux1:
+  assumes a0:"xins = [Ppushl_r x64Syntax.RCX, Ppopl x64Syntax.RCX]" and 
+          a1:"result = (exec_instr (xins!0) 1 reg m)"
+        shows "result = Next reg' m' \<longrightarrow> storev M32 m (sub64 (reg (IR SP)) (vlong_of_memory_chunk M32)) (reg (IR ireg.RCX)) \<noteq> None"
+proof (rule ccontr)
+  assume a2:"\<not> (result = Next reg' m' \<longrightarrow> storev M32 m (sub64 (reg (IR SP)) (vlong_of_memory_chunk M32)) (reg (IR ireg.RCX)) \<noteq> None)"
+  let ?tmp = "storev M32 m (sub64 (reg (IR SP)) (vlong_of_memory_chunk M32)) (reg (IR ireg.RCX)) "
+  let ?res_ok = "Next reg' m'"
+  have a3:"\<not> (\<not> result = ?res_ok \<or> (?tmp \<noteq> None))" using imp_conv_disj a2 by blast
+  have a4:"result = ?res_ok \<and> ?tmp = None" using a3 by simp
+   then show "False"
+   proof
+     have b0:"?tmp = None" using a4 conjE by simp
+     have b2: "exec_push 1 M32 m reg (reg (IR x64Syntax.RCX)) = Stuck"using a0 exec_instr_def 
+       by (simp add: b0 exec_push_def)
+     thus "False" using b2 
+       using a1 a4 by (simp add: a0 exec_instr_def)
+   qed
+ qed
+
+lemma push_pop_subgoal_rr_aux2_1:
+  assumes a0:"xins = [Ppushl_r x64Syntax.RCX, Ppopl x64Syntax.RCX]" and 
+    a1:"Next reg' m' = (exec_instr (xins!0) 1 reg m) " and
+    a2:"Next reg'' m'' = (exec_instr (xins!1) 1 reg' m') "
+  shows "reg'' (IR x64Syntax.RCX) = reg (IR x64Syntax.RCX)"
+proof -
+  have b0:"Next reg' m' = exec_push 1 M32 m reg (reg (IR x64Syntax.RCX))" using exec_instr_def by (simp add: a0 a1)
+  have b1:"Next reg' m' =
+    (case storev M32 m (sub64 (reg (IR SP)) (vlong_of_memory_chunk M32)) (reg (IR ireg.RCX)) of None \<Rightarrow> Stuck
+     | Some (x::64 word \<Rightarrow> 8 word option option) \<Rightarrow>
+         Next
+          ((undef_regs [CR ZF, CR CF, CR PF, CR SF, CR OF] (reg(IR SP := sub64 (reg (IR SP)) (vlong_of_memory_chunk M32))))
+           (RIP := add64 (undef_regs [CR ZF, CR CF, CR PF, CR SF, CR OF] (reg(IR SP := sub64 (reg (IR SP)) (vlong_of_memory_chunk M32))) RIP) (Vlong ((1::64 word) + (1::64 word)))))
+          x) " using b0 nextinstr_nf_def nextinstr_def exec_push_def by metis
+  have b2_1:"(exec_instr (xins!0) 1 reg m) = Next reg' m' \<longrightarrow> storev M32 m (sub64 (reg (IR SP)) (vlong_of_memory_chunk M32)) (reg (IR ireg.RCX)) \<noteq> None" using push_pop_subgoal_rr_aux1 a0 a1 by blast
+  have b2_2:"storev M32 m (sub64 (reg (IR SP)) (vlong_of_memory_chunk M32)) (reg (IR ireg.RCX)) \<noteq> None" using b2_1 a1 by simp
+  have b2:"storev M32 m (sub64 (reg (IR SP)) (vlong_of_memory_chunk M32)) (reg (IR ireg.RCX))= Some m'" using b1 b2_2 by auto
+  have b3:"reg' (IR SP) = sub64 (reg (IR SP)) (vlong_of_memory_chunk M32)" using b1 b2 by auto
+  let "?sp" = "reg' (IR SP)"
+  have b4:"storev M32 m (reg' (IR SP)) (reg (IR ireg.RCX)) = Some m'" using b2 b3 by simp
+  have c0:"Next reg'' m'' = exec_pop (1::64 word) M32 m' reg' (IR ireg.RCX)" using exec_instr_def by (simp add: a0 a2)
+  have c2:"loadv M32 m' (reg' (IR SP)) = Some (reg (IR ireg.RCX))" using b4 store_load_consistency by simp
+  let "?v" = " (reg (IR ireg.RCX))"
+  have c3:" Next reg'' m'' =
+    (case loadv M32 m' (reg' (IR SP)) of None \<Rightarrow> Stuck
+     | Some (v::val) \<Rightarrow>
+         Next
+          ((undef_regs [CR ZF, CR CF, CR PF, CR SF, CR OF] (reg'(IR ireg.RCX := ?v, IR SP := add64 (reg' (IR SP)) (vlong_of_memory_chunk M32))))
+           (RIP := add64 (undef_regs [CR ZF, CR CF, CR PF, CR SF, CR OF] (reg'(IR ireg.RCX := ?v, IR SP := add64 (reg' (IR SP)) (vlong_of_memory_chunk M32))) RIP) (Vlong ((1::64 word) + (1::64 word)))))
+          m')" using nextinstr_nf_def nextinstr_def exec_pop_def c2 
+    using c0 by force
+  have c4:"reg''(IR ireg.RCX) = ?v" using exec_pop_def c2 c3 by auto
+  thus ?thesis using c4 by simp
+qed
+
+lemma push_pop_subgoal_rr_aux2_2:
+  assumes a0:"xins = [Ppushl_r x64Syntax.RCX, Ppopl x64Syntax.RCX]" and 
+    a1:"Next reg'' m'' = interp2 n xins (Next reg m)" and
+    a2:"storev M32 m (sub64 (reg (IR SP)) (vlong_of_memory_chunk M32)) (reg (IR ireg.RCX)) \<noteq> None "
+  shows "reg'' (IR x64Syntax.RCX) = reg (IR x64Syntax.RCX)"
+proof-
+  have b0:"length xins = (2::nat)" using a0 by simp
+  thus ?thesis using b0 a0 a1 a2 push_pop_subgoal_rr_aux2_1 shift_subgoal_rr_aux1_1
+    by metis
+qed
+
+lemma shift_subgoal_rr_aux4_1:
+  assumes a0:"xins = [Ppushl_r x64Syntax.RCX, Pmovq_rr src (x64Syntax.RCX),Pshlq_r dst, Ppopl x64Syntax.RCX]" and 
+    a1:"Next reg'' m'' = interp2 n xins (Next reg m)" and
+    a2:"storev M32 m (sub64 (reg (IR SP)) (vlong_of_memory_chunk M32)) (reg (IR ireg.RCX)) \<noteq> None "
+  shows "reg'' (IR x64Syntax.RCX) = reg (IR x64Syntax.RCX)"
+proof-
+  have b0:"length xins = (4::nat)" using a0 by simp
+  thus ?thesis using b0 a0 a1 a2 push_pop_subgoal_rr_aux2_1 shift_subgoal_rr_aux1_1
+    sorry
+qed
+
+
+
+(*proof-
+  from a0 a2 have "\<exists> reg' m'. Next reg' m' = exec_push 1 M32 m reg (reg (IR x64Syntax.RCX))" 
+    using exec_instr_def push_pop_subgoal_rr_aux2_1 
+    using a3 exec_push_def by force
+  then obtain reg' m' where d0:" Next reg' m' = exec_push 1 M32 m reg (reg (IR x64Syntax.RCX))" by auto
+  thus ?thesis using d0 push_pop_subgoal_rr_aux2_1 shift_subgoal_rr_aux1_1 try
+*)
+
+
+(*sp consisency*)
+(*  let "?sp'"= "add64 (reg' (IR SP)) (vlong_of_memory_chunk M32)"
+  have c1:"?sp' = reg (IR SP)" using add64_def sub64_def sorry*)
+
+
+lemma shift_subgoal_rr_aux4_2:"xins = [Pmovq_rr src (x64Syntax.RCX),Pshlq_r dst] \<Longrightarrow> 
+    Next reg'' m'' = interp2 n xins (Next reg m) \<Longrightarrow> 
+    \<forall> r . r \<notin> {dst,x64Syntax.RCX} \<longrightarrow> reg' (IR r) = reg (IR r)"
+  sorry
+
+lemma shift_subgoal_rr_aux4:"xins = [Ppushl_r x64Syntax.RCX, Pmovq_rr src (x64Syntax.RCX),Pshlq_r dst,Ppopl x64Syntax.RCX] \<Longrightarrow> 
+    Next reg'' m'' = interp2 n xins (Next reg m) \<Longrightarrow> 
+    \<forall> r\<noteq>dst. reg' (IR r) = reg (IR r)"
+  sorry
+
+
+lemma shift_subgoal_rr_aux5:
+     "bins = BPF_ALU64 BPF_LSH dst (SOReg src) \<Longrightarrow>
+     xins = [Ppushl_r x64Syntax.RCX, Pmovq_rr ri (x64Syntax.RCX),Pshlq_r rd,Ppopl x64Syntax.RCX] \<Longrightarrow>
+     (BPF_OK pc rs' m' ss' is_v1 (cur_cu+1) remain_cu) = step fuel bins rs m ss is_v1 cur_cu remain_cu \<Longrightarrow>
+     Next reg' m' = interp2 sz xins (Next reg m) \<Longrightarrow>
+     rd = (bpf_to_x64_reg dst) \<Longrightarrow>
+     ri = (bpf_to_x64_reg src) \<Longrightarrow>
+     reg (IR rd) = Vlong n1 \<Longrightarrow>
+     reg (IR ri) = Vlong n2 \<Longrightarrow>
+     n1  = rs dst \<Longrightarrow>
+     n2  = rs src \<Longrightarrow> 
+     Vlong (rs' dst) = reg' (IR (bpf_to_x64_reg dst))"
+  sorry
+
+lemma shift_subgoal_rr_aux6:"
+    bins = BPF_ALU64 BPF_LSH dst (SOReg src) \<Longrightarrow> (BPF_OK pc rs' m' ss' is_v1 (cur_cu+1) remain_cu) = step fuel bins rs m ss is_v1 cur_cu remain_cu \<Longrightarrow>
+    \<forall> r \<noteq> dst. rs' r = rs r"
+  apply(cases "bins",simp_all)
+  apply(unfold eval_alu64_def,simp)
+  by (unfold eval_alu64_aux2_def, simp_all)
+
+lemma test1:
+  assumes 
+       a1:"Some bl = x64_encode (Porq_rr dst src)" and
+       a2:"list_in_list bl (unat pc) l_bin" and
+       a3:"x64_decode (unat pc) l_bin = Some (length l_bin, xins)"  
+     shows "xins = Porq_rr dst src"
+  using x64_encode_decode_consistency 
+  by (metis a1 a2 a3 option.sel prod.inject)
+
+value "x64_decodes 2 (Option.the(x64_encodes_suffix ([Pmovq_rr x64Syntax.RAX x64Syntax.RBX,Pnop])))"
+value "x64_decodes 0 (Option.the(x64_encodes_suffix ([Pnop,Pnop])))"
+value "map snd [(1::nat,Pnop),(3::nat,Pmovq_rr x64Syntax.RAX x64Syntax.RBX)]"
+
+
+value "x64_encodes_suffix [Pmovq_rr src dst,Pmovq_rr src dst]"
+value "x64_decodes 0 (Option.the(x64_encodes_suffix [Ppushl_r x64Syntax.RCX, Pmovq_rr (x64Syntax.RAX) (x64Syntax.RCX),
+  Pshlq_r (x64Syntax.RBX),Ppopl x64Syntax.RCX]))"
+value "x64_decodes 0 (Option.the(x64_encodes_suffix [Ppushl_r x64Syntax.RCX, Pmovq_rr (bpf_to_x64_reg src) (x64Syntax.RCX),
+Pshlq_r (bpf_to_x64_reg dst),Ppopl x64Syntax.RCX]))"
+
+lemma test2:
+  assumes 
+       a1:"Some bl = x64_encodes_suffix [Pnop]" and
+       a2:"list_in_list bl 0 l_bin" and
+       a3:"x64_decodes 0 l_bin = Some v" and
+       a4:"xins = map snd v"  
+     shows "xins = [Pnop]"
+  using x64_encodes_decodes_consistency a1 a2 a3 a4 by simp
+
+
+lemma shlq_subgoal_rr_generic:
+  assumes a0:"bins = BPF_ALU64 BPF_LSH dst (SOReg src)" and
+       a1:"per_jit_shift_reg64 4 dst src = Some bl" and
+       a2:"list_in_list bl (unat pc) l_bin" and
+       a3:"x64_decodes (unat pc) l_bin = Some v" and
+       a4:"(BPF_OK pc rs' m' ss' is_v1 (cur_cu+1) remain_cu) = step fuel bins rs m ss is_v1 cur_cu remain_cu" and
+       a5:"Next reg' m' = interp2 (unat pc) xins (Next reg m) " and
+       a6:"(\<forall> r. Vlong (rs r) = reg (IR (bpf_to_x64_reg r)))" and
+       a7:"(bpf_to_x64_reg dst) \<noteq> x64Syntax.RCX" and
+       a8:"xins = map snd v"
+  shows "(\<forall> r. Vlong (rs' r) = reg' (IR (bpf_to_x64_reg r)))"
+proof -
+  have b:"Some bl = x64_encodes_suffix [Ppushl_r x64Syntax.RCX, Pmovq_rr (bpf_to_x64_reg src) (x64Syntax.RCX),Pshlq_r (bpf_to_x64_reg dst),Ppopl x64Syntax.RCX]" 
+    using a0 a1 a7 per_jit_shift_reg64_def by simp
+  moreover have b0:"xins = [Ppushl_r x64Syntax.RCX, Pmovq_rr (bpf_to_x64_reg src) (x64Syntax.RCX),Pshlq_r (bpf_to_x64_reg dst),Ppopl x64Syntax.RCX]" 
+    using x64_encodes_decodes_consistency per_jit_shift_reg64_def a1 a2 a3 
+    using a8 calculation by presburger
+    moreover have b1:"Vlong (rs dst) = reg (IR (bpf_to_x64_reg dst))" using a6 spec by simp
+    moreover have b2:"Vlong (rs src) = reg (IR (bpf_to_x64_reg src))" using a6 spec by simp
+    hence b3:"Vlong (rs' dst) = reg' (IR (bpf_to_x64_reg dst))" using shift_subgoal_rr_aux5 b0 b1 b2 a0 a4 a5 by force
+    have b4:"\<forall> r \<noteq> dst. reg'(IR (bpf_to_x64_reg r)) = reg (IR (bpf_to_x64_reg r))" using b0 a5 shift_subgoal_rr_aux4 by simp
+    have b5:"\<forall> r \<noteq> dst. Vlong (rs' r) = Vlong (rs r)" using a0 a4 shift_subgoal_rr_aux6 by blast
+    have b6:"\<forall> r \<noteq> dst. Vlong (rs r) = reg (IR (bpf_to_x64_reg r))" using a6 by blast
+    have b7:"(\<forall> r \<noteq> dst. Vlong (rs' r) = reg' (IR (bpf_to_x64_reg r)))" by(simp add:b4 b5 b6) 
+    thus ?thesis using b3 by fastforce
+  qed
+
+
+
+ (*Vlong (rs (BPC)) = reg PC \<Longrightarrow>*)
+(*lemma ja_subgoal_aux1:
+      "bins = BPF_JA off \<Longrightarrow>
+       xins = Pjmp d \<Longrightarrow>
+       (BPF_OK pc rs' m' ss' is_v1 (cur_cu+1) remain_cu) = step fuel bins rs m ss is_v1 cur_cu remain_cu \<Longrightarrow>
+       Next reg' m' = exec_instr xins sz reg m \<Longrightarrow> 
+       d = ucast(off::i16)\<Longrightarrow>
+       pc = reg' PC"
+  apply (unfold exec_instr_def step)
+  apply simp
+  apply (unfold eval_pc_def nextinstr_def add64_def)
+  apply(simp_all)
+  apply(erule conjE)+
+  apply(cases "reg RIP", simp_all)
+  using cast_lemma4 by auto
+*)
+
+lemma ja_subgoal_aux2:"xins = Pjmp d \<Longrightarrow> Next reg' m' = exec_instr xins sz reg m \<Longrightarrow>
+       \<forall> r. reg' (IR (bpf_to_x64_reg r)) = reg (IR (bpf_to_x64_reg r))"
+  apply(unfold exec_instr_def, cases "xins", simp_all)
+  apply(unfold nextinstr_nf_def nextinstr_def add64_def) 
+  by auto
+
+lemma ja_subgoal_aux3:"bins = BPF_JA off \<Longrightarrow> (BPF_OK pc rs' m' ss' is_v1 cur_cu remain_cu) = step fuel bins rs m ss is_v1 cur_cu remain_cu \<Longrightarrow>
+       \<forall> r. rs' r = rs r"
+  by(cases "bins",simp_all)
+
+lemma ja_subgoal_generic:
+  assumes a0:"bins = BPF_JA off" and
+       a1:"per_jit_ja (ucast off) = Some bl" and
+       a2:"list_in_list bl (unat pc) l_bin" and
+       a3:"x64_decode (unat pc) l_bin = Some (length l_bin, xins)" and
+       a4:"(BPF_OK pc rs' m' ss' is_v1 (cur_cu+1) remain_cu) = step fuel bins rs m ss is_v1 cur_cu remain_cu" and
+       a5:"Next reg' m' = exec_instr xins sz reg m" and
+       a6:"(\<forall> r. Vlong (rs r) = reg (IR (bpf_to_x64_reg r)))" 
+  shows "(\<forall> r. Vlong (rs' r) = reg' (IR (bpf_to_x64_reg r)))"
+proof -
+  have b0:"xins = Pjmp (ucast off)" using x64_encode_decode_consistency per_jit_ja_def a1 a2 a3 get_relative_offset_def by fastforce
+  moreover have b2:"(\<forall> r. Vlong (rs r) = reg (IR (bpf_to_x64_reg r)))" using a6 by simp
+    have b4:"\<forall> r. reg'(IR (bpf_to_x64_reg r)) = reg (IR (bpf_to_x64_reg r))" using b0 a5 ja_subgoal_aux2 by simp
+    have b5:"\<forall> r. Vlong (rs' r) = Vlong (rs r)" using a0 a4 ja_subgoal_aux3 by simp
+    have b6:"\<forall> r. Vlong (rs r) = reg (IR (bpf_to_x64_reg r))" using a6 by blast
+    have b7:"(\<forall> r. Vlong (rs' r) = reg' (IR (bpf_to_x64_reg r)))" by(simp add:b4 b5 b6) 
+    thus ?thesis using b7 by fastforce
+  qed
+
 
 lemma load_subgoal_aux1:
       "bins = BPF_LDX chk dst src (b_off::i16) \<Longrightarrow>
@@ -244,7 +725,7 @@ proof (rule ccontr)
        n1  = rs dst \<Longrightarrow>
        n2  = rs src \<Longrightarrow>
        b_off = scast x_off \<Longrightarrow>
-       (BPF_OK rs' mem' ss'  is_v1 cur_cu remain_cu) = step  bins rs mem ss is_v1 cur_cu remain_cu \<Longrightarrow>
+       (BPF_OK pc rs' mem' ss' is_v1 cur_cu remain_cu) = step fuel bins rs mem ss is_v1 cur_cu remain_cu \<Longrightarrow>
        Next reg' m'  = exec_instr xins sz reg m \<Longrightarrow> 
        m = mem \<Longrightarrow>
        Mem.loadv chk mem (Vlong (eval_snd_op_u64 (SOReg src) rs + scast (scast b_off)))\<noteq> None \<Longrightarrow>
@@ -253,14 +734,12 @@ proof (rule ccontr)
   apply (unfold exec_instr_def step)
   apply(cases xins)
   apply simp_all
-  apply (unfold eval_load_def Let_def cast_lemma5, simp_all)
-apply (simp add: exec_load_def)
   apply (simp add: exec_load_def eval_addrmode64_def add64_def nextinstr_nf_def nextinstr_def)
   apply (cases "loadv chk mem (Vlong (rs src + scast x_off))")
    apply simp
   apply (cases "loadv chk mem (Vlong (rs src + scast (scast x_off)))")
   apply simp_all
-  using cast_lemma5  load_subgoal_aux2_1
+  using  load_subgoal_aux2_1
 *)
 
 
@@ -292,9 +771,12 @@ proof-
   have b3:"Next reg' m' = (case loadv chk m (eval_addrmode64 (?t) reg) 
            of None \<Rightarrow> Stuck | Some (v::val) \<Rightarrow> Next (nextinstr_nf sz (reg(IR (bpf_to_x64_reg dst) := v))) m) "
     using exec_load_def by (simp add: b2)
-  have b4:"Next reg' m' = (case loadv chk m (Vlong (rs src + scast x_off)) of None \<Rightarrow> Stuck
+  (*have b4:"Next reg' m' = (case loadv chk m (Vlong (rs src + scast x_off)) of None \<Rightarrow> Stuck
         | Some (v::val) \<Rightarrow> Next (nextinstr_nf sz (reg(IR (bpf_to_x64_reg dst) := v))) m)"
-    using eval_addrmode64_def b3 add64_def nextinstr_nf_def using a3 a5 a7 sorry
+    using eval_addrmode64_def b3 add64_def nextinstr_nf_def using a3 a5 a7 sorry*)
+  have b4:"Next reg' m' = (case loadv chk m (Vlong (rs src + scast x_off)) of None \<Rightarrow> Stuck | 
+    Some (v::val) \<Rightarrow> Next (nextinstr_nf sz (reg(IR (bpf_to_x64_reg dst) := v))) m)" 
+    using exec_load_def eval_addrmode64_def b3 add64_def nextinstr_nf_def nextinstr_def a3 a5 a7 a11 sorry
   have b5:"Next reg' m' = Next (nextinstr_nf sz (reg(IR (bpf_to_x64_reg dst) := Option.the(?tmp)))) m" using b4 b1 apply (cases "bins")
     apply simp_all using a0  apply simp_all using a8 option.sel sorry
   have b6:" reg'(IR (bpf_to_x64_reg dst)) = Option.the(?tmp)" using nextinstr_nf_def nextinstr_def b5 by simp
@@ -306,10 +788,10 @@ proof-
 (*
   fix v1 assume "?tmp = Some(Vlong v1)" 
   have c1_1:"(Option.the(?rss') dst) = v1" using a0 a9 the_def eval_load_def Let_def 
-    using \<open>loadv (chk) (mem) (Vlong (eval_snd_op_u64 (SOReg (src)) (rs) + scast (b_off))) = Some (Vlong (v1))\<close> by force
+    using loadv (chk) (mem) (Vlong (eval_snd_op_u64 (SOReg (src)) (rs) + scast (b_off))) = Some (Vlong (v1)) by force
   fix v2 assume "?tmp = Some(Vint v2)" 
   have c1_2:"(Option.the(?rss') dst) = ucast v2" using a0 a9 the_def eval_load_def Let_def 
-    using \<open>loadv (chk) (mem) (Vlong (eval_snd_op_u64 (SOReg (src)) (rs) + scast (b_off))) = Some (Vint (v2))\<close> by force
+    using loadv (chk) (mem) (Vlong (eval_snd_op_u64 (SOReg (src)) (rs) + scast (b_off))) = Some (Vint (v2)) by force
   fix v3 assume "?tmp = None" 
  *)
   have c1:"Vlong ((Option.the(?rss') dst)) = Option.the(?tmp)" (*using a0 a9 the_def eval_load_def Let_def c0 cast_lemma6*)
@@ -346,9 +828,7 @@ proof-
            then show ?thesis using c0 d1 by simp
        qed
      qed
-  have c2:" (BPF_OK pc rs' mem' ss is_v1 (cur_cu+1) remain_cu) = (BPF_OK ((Option.the(?rss'))#BPC <-- (1+ (Option.the(?rss') BPC))) mem ss  is_v1 cur_cu remain_cu) " 
-    using c0 Let_def a9 a0 by auto
-  have c3:"Option.the(?rss')dst = rs' dst" using the_def c2 by simp
+  have c3:"Option.the(?rss')dst = rs' dst" using the_def sorry
   have c4:"Vlong (rs' dst) = Option.the(?tmp)" using c3 c1 by simp
   thus ?thesis using c4 b6 by simp
 qed
@@ -410,115 +890,59 @@ proof -
     thus ?thesis using b3 by fastforce
   qed
 
-lemma subq_subgoal_rr_aux1:
-     "bins = BPF_ALU64 BPF_SUB dst (SOReg src) \<Longrightarrow>
-     xins = Psubq_rr rd ri \<Longrightarrow>
-     (BPF_OK pc rs' m' ss' is_v1 (cur_cu+1) remain_cu) = step fuel bins rs m ss is_v1 cur_cu remain_cu \<Longrightarrow>
-     Next reg' m'  = exec_instr xins sz reg m \<Longrightarrow>
-     rd = (bpf_to_x64_reg dst) \<Longrightarrow>
-     ri = (bpf_to_x64_reg src) \<Longrightarrow>
-     reg (IR rd) = Vlong n1 \<Longrightarrow>
-     reg (IR ri) = Vlong n2 \<Longrightarrow>
-     n1  = rs dst \<Longrightarrow>
-     n2  = rs src \<Longrightarrow> 
-     Vlong (rs' dst) = reg' (IR (bpf_to_x64_reg dst))"
+lemma addl_subgoal_rr:
+      "bins = BPF_ALU BPF_ADD dst (SOReg src) \<Longrightarrow>
+       xins = Paddl_rr rd ri \<Longrightarrow>
+       (BPF_OK pc rs' m' ss' is_v1 (cur_cu+1) remain_cu) = step fuel bins rs m ss is_v1 cur_cu remain_cu \<Longrightarrow>
+       Next reg' m'  = exec_instr xins sz reg m \<Longrightarrow> 
+       rd = bpf_to_x64_reg dst \<Longrightarrow>
+       ri = bpf_to_x64_reg src \<Longrightarrow>
+       reg (IR rd) = Vint n1 \<Longrightarrow>
+       reg (IR ri) = Vint n2 \<Longrightarrow>
+       ucast n1 = rs dst \<Longrightarrow>
+       ucast n2  = rs src \<Longrightarrow>
+       reg' (IR rd) = Vint n3 \<Longrightarrow>
+       ucast n3 = rs'dst"
   apply (unfold exec_instr_def step)
   apply simp
-  apply (unfold eval_alu64_def)
-  apply (cases BPF_SUB, simp_all)
-  apply (unfold eval_alu64_aux1_def)
+  apply (unfold eval_alu32_def)
+  apply (unfold eval_alu32_aux1_def)
   apply (unfold Let_def)
-  apply (cases BPF_SUB, simp_all)
-  apply (unfold sub64_def)
+  apply (unfold add64_def add32_def)
   apply (unfold nextinstr_nf_def nextinstr_def eval_reg_def)
-  by simp
-
-lemma subq_subgoal_rr_aux2_1:"xins = Psubq_rr dst src \<Longrightarrow> Next reg' m' = exec_instr xins sz reg m \<Longrightarrow> \<forall> r \<noteq> dst . reg' (IR r) = reg (IR r)"
-  apply(unfold exec_instr_def, cases "xins", simp_all)
-  apply(unfold nextinstr_nf_def nextinstr_def add64_def) 
-  by auto
-
-lemma subq_subgoal_rr_aux2_2:"xins = Psubq_rr (bpf_to_x64_reg dst) (bpf_to_x64_reg src) \<Longrightarrow> Next reg' m' = exec_instr xins sz reg m \<Longrightarrow>
-       \<forall> r \<noteq> bpf_to_x64_reg dst. reg' (IR r) = reg (IR r)"
-  using subq_subgoal_rr_aux2_1 by blast
-
-lemma subq_subgoal_rr_aux2:"xins = Psubq_rr (bpf_to_x64_reg dst) (bpf_to_x64_reg src) \<Longrightarrow> Next reg' m' = exec_instr xins sz reg m \<Longrightarrow>
-       \<forall> r \<noteq> dst. reg' (IR (bpf_to_x64_reg r)) = reg (IR (bpf_to_x64_reg r))"
-  using bpf_to_x64_reg_corr subq_subgoal_rr_aux2_2 by metis
+  apply simp
+  apply (unfold add64_def)
+  apply (erule conjE)
+  using cast_lemma2
+  
 
 
-lemma subq_subgoal_rr_aux3:"bins = BPF_ALU64 BPF_SUB dst (SOReg src) \<Longrightarrow> (BPF_OK pc rs' m' ss' is_v1 (cur_cu+1) remain_cu) = step fuel bins rs m ss is_v1 cur_cu remain_cu \<Longrightarrow>
-       \<forall> r \<noteq> dst. rs' r = rs r"
-  apply(cases "bins",simp_all)
-  apply(unfold eval_alu64_def,simp)
-  by (unfold eval_alu64_aux1_def, simp)
 
-lemma subq_subgoal_rr_generic:
-  assumes a0:"bins = BPF_ALU64 BPF_SUB dst (SOReg src)" and
-       a1:"per_jit_sub_reg64 dst src = Some bl" and
-       a2:"list_in_list bl (unat pc) l_bin" and
-       a3:"x64_decode (unat pc) l_bin = Some (length l_bin, xins)" and
-       a4:"(BPF_OK pc rs' m' ss' is_v1 (cur_cu+1) remain_cu) = step fuel bins rs m ss is_v1 cur_cu remain_cu" and
-       a5:"Next reg' m'  = exec_instr xins sz reg m" and
-       a6:"(\<forall> r. Vlong (rs r) = reg (IR (bpf_to_x64_reg r)))" 
-  shows "(\<forall> r. Vlong (rs' r) = reg' (IR (bpf_to_x64_reg r)))"
-proof -
-  have b0:"xins = Psubq_rr (bpf_to_x64_reg dst) (bpf_to_x64_reg src)" using x64_encode_decode_consistency per_jit_sub_reg64_def a1 a2 a3 by fastforce
-    moreover have b1:"Vlong (rs dst) = reg (IR (bpf_to_x64_reg dst))" using a6 spec by simp
-    moreover have b2:"Vlong (rs src) = reg (IR (bpf_to_x64_reg src))" using a6 spec by simp
-    hence b3:"Vlong (rs' dst) = reg' (IR (bpf_to_x64_reg dst))" using subq_subgoal_rr_aux1 b0 b1 b2 a0 a4 a5 by force
-    have b4:"\<forall> r \<noteq> dst. reg'(IR (bpf_to_x64_reg r)) = reg (IR (bpf_to_x64_reg r))" using b0 a5 subq_subgoal_rr_aux2 by simp
-    have b5:"\<forall> r \<noteq> dst. Vlong (rs' r) = Vlong (rs r)" using a0 a4 subq_subgoal_rr_aux3 by simp
-    have b6:"\<forall> r \<noteq> dst. Vlong (rs r) = reg (IR (bpf_to_x64_reg r))" using a6 by blast
-    have b7:"(\<forall> r \<noteq> dst. Vlong (rs' r) = reg' (IR (bpf_to_x64_reg r)))" by(simp add:b4 b5 b6) 
-    thus ?thesis using b3 by fastforce
-  qed
-
- (*Vlong (rs (BPC)) = reg PC \<Longrightarrow>*)
-(*lemma ja_subgoal_aux1:
-      "bins = BPF_JA off \<Longrightarrow>
-       xins = Pjmp d \<Longrightarrow>
+lemma addl_subgoal_ri:
+      "bins = BPF_ALU BPF_ADD dst (SOImm src) \<Longrightarrow>
+       xins = Paddl_ri rd imm \<Longrightarrow>
        (BPF_OK pc rs' m' ss' is_v1 (cur_cu+1) remain_cu) = step fuel bins rs m ss is_v1 cur_cu remain_cu \<Longrightarrow>
        Next reg' m' = exec_instr xins sz reg m \<Longrightarrow> 
-       d = ucast(off::i16)\<Longrightarrow>
-       pc = reg' PC"
+       rd = bpf_to_x64_reg dst \<Longrightarrow>
+       imm = ucast (src) \<Longrightarrow>
+       reg (IR rd) = Vint n1 \<Longrightarrow>
+       ucast n1  = rs dst \<Longrightarrow>
+       reg' (IR rd) = Vint n3 \<Longrightarrow>
+       ucast n3 = rs'dst"
   apply (unfold exec_instr_def step)
   apply simp
-  apply (unfold eval_pc_def nextinstr_def add64_def)
-  apply(simp_all)
-  apply(erule conjE)+
-  apply(cases "reg RIP", simp_all)
-  using cast_lemma4 by auto
-*)
-
-lemma ja_subgoal_aux2:"xins = Pjmp d \<Longrightarrow> Next reg' m' = exec_instr xins sz reg m \<Longrightarrow>
-       \<forall> r. reg' (IR (bpf_to_x64_reg r)) = reg (IR (bpf_to_x64_reg r))"
-  apply(unfold exec_instr_def, cases "xins", simp_all)
-  apply(unfold nextinstr_nf_def nextinstr_def add64_def) 
-  by auto
-
-lemma ja_subgoal_aux3:"bins = BPF_JA off \<Longrightarrow> (BPF_OK pc rs' m' ss' is_v1 cur_cu remain_cu) = step fuel bins rs m ss is_v1 cur_cu remain_cu \<Longrightarrow>
-       \<forall> r. rs' r = rs r"
-  by(cases "bins",simp_all)
-
-lemma ja_subgoal_generic:
-  assumes a0:"bins = BPF_JA off" and
-       a1:"per_jit_ja (ucast off) = Some bl" and
-       a2:"list_in_list bl (unat pc) l_bin" and
-       a3:"x64_decode (unat pc) l_bin = Some (length l_bin, xins)" and
-       a4:"(BPF_OK pc rs' m' ss' is_v1 (cur_cu+1) remain_cu) = step fuel bins rs m ss is_v1 cur_cu remain_cu" and
-       a5:"Next reg' m' = exec_instr xins sz reg m" and
-       a6:"(\<forall> r. Vlong (rs r) = reg (IR (bpf_to_x64_reg r)))" 
-  shows "(\<forall> r. Vlong (rs' r) = reg' (IR (bpf_to_x64_reg r)))"
-proof -
-  have b0:"xins = Pjmp (ucast off)" using x64_encode_decode_consistency per_jit_ja_def a1 a2 a3 sorry
-  moreover have b2:"(\<forall> r. Vlong (rs r) = reg (IR (bpf_to_x64_reg r)))" using a6 by simp
-    have b4:"\<forall> r. reg'(IR (bpf_to_x64_reg r)) = reg (IR (bpf_to_x64_reg r))" using b0 a5 ja_subgoal_aux2 by simp
-    have b5:"\<forall> r. Vlong (rs' r) = Vlong (rs r)" using a0 a4 ja_subgoal_aux3 by simp
-    have b6:"\<forall> r. Vlong (rs r) = reg (IR (bpf_to_x64_reg r))" using a6 by blast
-    have b7:"(\<forall> r. Vlong (rs' r) = reg' (IR (bpf_to_x64_reg r)))" by(simp add:b4 b5 b6) 
-    thus ?thesis using b7 by fastforce
-  qed
+  apply (unfold eval_alu32_def)
+  apply (cases BPF_ADD, simp_all)
+  apply (unfold eval_alu32_aux1_def)
+  apply (unfold Let_def)
+  apply (cases BPF_ADD, simp_all)
+  apply (unfold add64_def add32_def)
+  apply (unfold nextinstr_nf_def nextinstr_def eval_reg_def)
+  apply simp
+  apply (unfold add64_def)
+  apply (erule conjE)
+  using cast_lemma2 
+  by metis
 
 
 lemma subl_subgoal_ri:
@@ -548,49 +972,5 @@ lemma subl_subgoal_ri:
   apply (cases "is_v1", simp_all)
   using cast_lemma2 
   sorry
-
-
-lemma movq_subgoal_rr:
-      "bins = BPF_ALU64 BPF_MOV dst (SOReg src) \<Longrightarrow>
-       xins = Pmovq_rr rd ri \<Longrightarrow>
-       (BPF_OK pc rs' m' ss' is_v1 (cur_cu+1) remain_cu) = step fuel bins rs m ss is_v1 cur_cu remain_cu \<Longrightarrow>
-       Next reg' m'  = exec_instr xins sz reg m \<Longrightarrow> 
-       rd = bpf_to_x64_reg dst \<Longrightarrow>
-       ri = bpf_to_x64_reg src \<Longrightarrow>
-       reg (IR rd) = Vlong n1 \<Longrightarrow>
-       reg (IR ri) = Vlong n2 \<Longrightarrow>
-       n1  = rs dst \<Longrightarrow>
-       n2  = rs src \<Longrightarrow>
-       reg' (IR rd) = Vlong n3 \<Longrightarrow>
-       ucast n3 = rs'dst"
-(*memory_mapping bstate = m' \<and> (reg' (IR rd)) = Vlong (rs'dst)"*)
-  apply (unfold exec_instr_def step)
-  apply simp
-  apply (unfold eval_alu64_def)
-  apply (unfold eval_alu64_aux1_def)
-  apply (unfold Let_def)
-  apply (unfold nextinstr_nf_def nextinstr_def eval_reg_def)
-  by simp
-
-lemma movq_subgoal_ri:
-      "bins = BPF_ALU64 BPF_MOV dst (SOImm src) \<Longrightarrow>
-       xins = Pmovq_ri rd imm \<Longrightarrow>
-       (BPF_OK pc rs' m' ss' is_v1 (cur_cu+1) remain_cu) = step fuel bins rs m ss is_v1 cur_cu remain_cu \<Longrightarrow>
-       Next reg' m' = exec_instr xins sz reg m \<Longrightarrow> 
-       rd = bpf_to_x64_reg dst \<Longrightarrow>
-       imm = ucast (src) \<Longrightarrow>
-       reg (IR rd) = Vlong n1 \<Longrightarrow>
-       ucast n1  = rs dst \<Longrightarrow>
-       reg' (IR rd) = Vlong n3 \<Longrightarrow>
-       ucast n3 = rs'dst"
-  apply (unfold exec_instr_def step)
-  apply simp
-  apply (unfold eval_alu64_def)
-  apply (cases BPF_MOV, simp_all)
-  apply (unfold nextinstr_def)
-  apply (erule conjE)
-  try
-  apply(unfold eval_alu64_aux1_def add64_def) 
-  by simp
 
 end
