theory/x64DecodeProof.thy
@@ -52,14 +52,19 @@ declare if_split_asm [split]
   apply(simp split del:if_split)
 *)
 
-
 lemma x64_encode_decode_consistency:
   "list_in_list l_bin pc l \<Longrightarrow> Some l_bin = x64_encode ins \<Longrightarrow>
     x64_decode pc l = Some (length l_bin, ins)"
   sorry
+
+lemma x64_encodes_decodes_consistency:
+  "list_in_list l_bin pc l \<Longrightarrow> Some l_bin = x64_encodes_suffix insns \<Longrightarrow>
+    x64_decodes pc l = Some v \<Longrightarrow> insns = map snd v"
+  sorry
+  (*using  x64_encode_decode_consistency x64_decodes_def x64_encodes_suffix_def x64_encodes_def *)
  (* 
  apply (cases ins; simp_all)
-
+                                                                                                  
   subgoal for dst src
   \<comment> \<open> Pmovl_rr \<close> 
     apply (unfold Let_def)
