theory/x64Syntax.thy
@@ -230,7 +230,7 @@ datatype instruction =
   | Pxorq_rr ireg ireg
   | Pxorl_ri ireg u32
   | Pshll_ri ireg u8
-  | Pshlq_ri ireg u8
+  | Pshlq_ri ireg u8                         
   | Pshll_r ireg
   | Pshlq_r ireg
   | Pshrl_ri ireg u8
